%
%
The three step transitional probabilities are given as,
\begin{align}
    P(X_3 = j \: | \: X_0 = i) = P(X_{n+3} = j \: | \: X_n = i) = \nonumber \\
    (\vec{P}^3)_{ij} \: for \: any \: n
\end{align}

\begin{align} \label{eq:solutions/2017/dec/51/eq:3_1}
    \vec{P}^3 = \myvec{0 & \frac{1}{2} & \frac{1}{2} \\
    \frac{1}{2} & 0 & \frac{1}{2} \\
    \frac{1}{2} & \frac{1}{2} & 0}^3 = 
    \myvec{\frac{1}{4} & \frac{3}{8} & \frac{3}{8} \\
    \frac{3}{8} & \frac{1}{4} & \frac{3}{8} \\
    \frac{3}{8} & \frac{3}{8} & \frac{1}{4}}
\end{align}
From \eqref{eq:solutions/2017/dec/51/eq:3_1},
\begin{align}
    P(X_3 = 1 \: | \: X_0 = 1) = (\vec{P}^3)_{11} = \frac{1}{4}
\end{align}
